############
# author: Kent O'Sullivan
# purpose: The Cyber Simulation Terrain is the Independent Network Model use to support the CESO in representing Cyber Effects
# worldview: Assumes omniscience of modelled network. View is focused on describing connections and interrelations. 
# If you use this work please reference: 
# O’Sullivan, K and Turnbull, B (2015). The Cyber Simulation Terrain: Towards an Open Source Cyber Effects Simulation Ontology. Accepted for the 16th Australian Information Warfare Conference in Perth, Western Australia, Australia 30 Nov – 02 Dec. 
############

#     _______     ______  ______ _____     _____ _____ __  __ _    _ _            _______ _____ ____  _   _   _______ ______ _____  _____            _____ _   _ 
#    / ____\ \   / /  _ \|  ____|  __ \   / ____|_   _|  \/  | |  | | |        /\|__   __|_   _/ __ \| \ | | |__   __|  ____|  __ \|  __ \     /\   |_   _| \ | |
#   | |     \ \_/ /| |_) | |__  | |__) | | (___   | | | \  / | |  | | |       /  \  | |    | || |  | |  \| |    | |  | |__  | |__) | |__) |   /  \    | | |  \| |
#   | |      \   / |  _ <|  __| |  _  /   \___ \  | | | |\/| | |  | | |      / /\ \ | |    | || |  | | . ` |    | |  |  __| |  _  /|  _  /   / /\ \   | | | . ` |
#   | |____   | |  | |_) | |____| | \ \   ____) |_| |_| |  | | |__| | |____ / ____ \| |   _| || |__| | |\  |    | |  | |____| | \ \| | \ \  / ____ \ _| |_| |\  |
#    \_____|  |_|  |____/|______|_|  \_\ |_____/|_____|_|  |_|\____/|______/_/    \_\_|  |_____\____/|_| \_|    |_|  |______|_|  \_\_|  \_\/_/    \_\_____|_| \_|
#                                                                                                                                                                                                                                                                                                                                                                                                                                                                                                                                                                                                                                                                                                                                                                                                                                                                                   

@prefix core:    	<http://www.accs.unsw.adfa.edu.au/2015/09/05/core/core#> .
@prefix cst:   		<http://www.accs.unsw.adfa.edu.au/2015/09/05/domain/cyber/CyberSimulationTerrain/cst#> .

@prefix rdf:     	<http://www.w3.org/1999/02/22-rdf-syntax-ns#> .
@prefix xsd:     	<http://www.w3.org/2001/XMLSchema#> .
@prefix rdfs:    	<http://www.w3.org/2000/01/rdf-schema#> .
@prefix owl:		<http://www.w3.org/2002/07/owl#> .

#     ____   _          _      ____    ____    _____   ____  
#    / ___| | |        / \    / ___|  / ___|  | ____| / ___| 
#   | |     | |       / _ \   \___ \  \___ \  |  _|   \___ \ 
#   | |___  | |___   / ___ \   ___) |  ___) | | |___   ___) |
#    \____| |_____| /_/   \_\ |____/  |____/  |_____| |____/ 
#                                                            

#Classes relating to basic nodes and connection 

cst:Node 
	rdf:type rdfs:Class ;
	rdfs:comment "A node on a network. SuperClass, use subClasses where appropriate"^^xsd:string ;
	rdfs:label "Network Node"^^xsd:string .

cst:Computer
  	rdf:type rdfs:Class ;
  	rdfs:comment "Computer object"^^xsd:string ;
  	rdfs:label "Computer"^^xsd:string ;
  	rdfs:subClassOf cst:Node .

 cst:Router
  	rdf:type rdfs:Class ;
  	rdfs:comment "Router is a specialised type of computer for routing traffic between networks."^^xsd:string ;
  	rdfs:label "Router"^^xsd:string ;
  	rdfs:subClassOf cst:Computer .

cst:Nic
	rdf:type rdfs:Class ;
	rdfs:comment "Component of computer that enables network connectivity. Computer can have 0 to many. Has MAC and IP properties."^^xsd:string ;
	rdfs:label "Network Interface Card"^^xsd:string .	


# Classes relating to Networking and comminications between nodes

cst:Network
	rdf:type rdfs:Class ;
	rdfs:comment "Collection of computer objects. Has a Unique Name"^^xsd:string ;
	rdfs:label "Network"^^xsd:string .

cst:SubNetwork
	rdf:type rdfs:Class ;
	rdfs:comment "Collection of computer objects. Used to connect endpoint workstations"^^xsd:string ;
	rdfs:label "SubNetwork"^^xsd:string ;
	rdfs:subClassOf cst:Network .

cst:InterNetwork
	rdf:type rdfs:Class ;
	rdfs:comment "Collection of ROUTER objects. USed to connect disparate networks"^^xsd:string ;
	rdfs:label "InterNetwork"^^xsd:string ;
	rdfs:subClassOf cst:Network .

cst:Route 
	rdf:type rdfs:Class ;
	rdfs:comment "Path from one network edge node to another within a router. Has properties of routeNumber, From and To"^^xsd:string ;
	rdfs:label "Route"^^xsd:string .

cst:Internet 
	rdf:type rdfs:Class ;
	rdfs:comment "Internet is a per-node property. If a Node with a NIC is connected to a subnet with an edgeNic conected to a router with a route to the internet which is connected to the internet then internet connectivity is inferred. "^^xsd:string ;
	rdfs:label "Internet"^^xsd:string ;
	rdfs:subClassOf cst:Network .		


#Classes to do with Wireless

cst:WirelessAccessPoint
	rdf:type rdfs:Class ;
	rdfs:comment "Wireless access point will permit wireless access to a conected subnet. Will have an associated Wireless Encryption Standard"^^xsd:string ;
	rdfs:label "Wireless Access Point" .

cst:WirelessSecurityProtocol
	rdf:type rdfs:Class ;
	rdfs:comment "Security Protocol used to protect a wireless network. Will have A type and a strength."^^xsd:string ;
	rdfs:label "Wireless Security Protocol" .


cst:WirelessNic
	rdf:type rdfs:Class ;
	rdfs:comment "Component of computer that enables wireless network connectivity. Computer can have 0 to many. Has MAC and IP properties."^^xsd:string ;
	rdfs:label "Wireless Network Interface Card"^^xsd:string ;	
	rdfs:subClassOf cst:Nic .


#Classes to Do with Virtualisation

cst:VirtualNetwork
	rdf:type rdfs:Class ;
	rdfs:comment "Collection of Virtual computer objects. Used to connect virtual machines to each other and to physical workstations"^^xsd:string ;
	rdfs:label "Virtual Network"^^xsd:string ;
	rdfs:subClassOf cst:Network .	

cst:VirtualNic
	rdf:type rdfs:Class ;
	rdfs:comment "Component of computer that enables network connectivity with a virtual machine. Virtual machines MUST use a VNic. Physical machines must have a VNIC to interact with Virtual machine. Has MAC and IP properties."^^xsd:string ;
	rdfs:label "Virtual Network Interface Card"^^xsd:string ;	
	rdfs:subClassOf cst:Nic .	

 cst:VirtualMachine
  	rdf:type rdfs:Class ;
  	rdfs:comment "A virtual Computer Object. Must be hosted on a physical computer ."^^xsd:string ;
  	rdfs:label "Virtual Machine"^^xsd:string ;
  	rdfs:subClassOf cst:Node .


# The follwoing Classes relate to software and services. 

cst:SoftwareType
	rdf:type rdfs:Class ;
	rdfs:comment "Software Class - use to define applications or operating systems. Use InstalledSoftwareVersion to Instantiate to a Node"^^xsd:string ;
	rdfs:label "Software Type"^^xsd:string .

cst:InstalledSoftwareVersion
	rdf:type rdfs:Class ;
	rdfs:comment "Used to define a particular version of software. Will operate as a particular privilege level. Has a version number. Runs on a node."^^xsd:string ;
	rdfs:label "Installed Software Version"^^xsd:string .

cst:SoftwareVulnerability
	rdf:type rdfs:Class ;
	rdfs:comment "Enumerates a vulnerability in a particular software version. Will have a CVE ID. "^^xsd:string ;
	rdfs:label "Software Vulnerability"^^xsd:string .

cst:SoftwareWeakness
	rdf:type rdfs:Class ;
	rdfs:comment "Categorisation of Vulnerability into an area of weakness based on CWE. Links to the Vulnerability CVE."^^xsd:string ;
	rdfs:label "Software Weakness"^^xsd:string .

cst:Service 
	rdf:type rdfs:Class ;
	rdfs:comment "The manifestation of a running software version on a computer system (SuperClass - use subClasses)"^^xsd:string ;
	rdfs:label "Service"^^xsd:string .

cst:LocalService
	rdf:type rdfs:Class ;
	rdfs:comment "A Service local to a computer system with no network projection. Inherits privilege level from parent Class. "^^xsd:string ;
	rdfs:label "Local Service"^^xsd:string ;
	rdfs:subClassOf cst:Service .

cst:RemoteService 	
	rdf:type rdfs:Class ;
	rdfs:comment "A Service accessible remotely - projects itself over a NIC to a network on a port"^^xsd:string ;
	rdfs:label "Remote Service"^^xsd:string ;
	rdfs:subClassOf cst:Service .

cst:SoftwareConfiguration
	rdf:type rdfs:Class ;
	rdfs:comment "A configuration item specific to a piece of software."^^xsd:string ;
	rdfs:label "Software Configuration"^^xsd:string .	


# The Following Classes are to Do with Domains and Users

cst:Domain 
	rdf:type rdfs:Class ;
	rdfs:comment "A Domain is a distinct collection of computers, subnets and peripherals sharing the same domain name and sharing resources."^^xsd:string ;
	rdfs:label "Domain" .

cst:DomainController
	rdf:type rdfs:Class ;
	rdfs:comment "Special Instance of a Node - enables a domain to exist on any subnet it is linked to. Will still be a member of a subnet. If domain has multiple subnets, subordinate, nested subents will be used."^^xsd:string ;
	rdfs:label "Domain Controller"^^xsd:string ;
	rdfs:subClassOf cst:Node .

cst:User
	rdf:type rdfs:Class ;
	rdfs:comment "The Virtual Persona of a physical user. Used to control access to resources and authentication. Users will have an ID, Username and Password. SuperClass, Use SubClasses"^^xsd:string ;
	rdfs:label "User"^^xsd:string .

cst:DomainUser
	rdf:type rdfs:Class ;
	rdfs:comment "User account on a given domain"^^xsd:string ;
	rdfs:label "Domain User"^^xsd:string ;
	rdfs:subClassOf cst:User .

cst:LocalUser
	rdf:type rdfs:Class ;
	rdfs:comment "User account on a given domain"^^xsd:string ;
	rdfs:label "Local User"^^xsd:string ;
	rdfs:subClassOf cst:User .


##The Following Classes are to do with data, disks and encryption 

cst:Disk 
	rdf:type rdfs:Class ;
	rdfs:comment "A Hard disk belonging to a computer. Used to Store Data. Includes HDD, SSD etc. Can have protections such as Encryption"^^xsd:string ;
	rdfs:label "Disk"^^xsd:string .

cst:Data 
	rdf:type rdfs:Class ;
	rdfs:comment "Data is the inforamation stored on a Disk. It is owned by a user and will be of a specific size and nature. Should refer onlt to user and application data Doesn't include program files etc."^^xsd:string ;
	rdfs:label "Data"^^xsd:string .	

cst:Encryption 
	rdf:type rdfs:Class ;
	rdfs:comment "Defines the types of at-rest disk encryption available to a disk"^^xsd:string ;
	rdfs:label "Encryption" .


#Classes Relating to IDS

cst:NetworkIDS 
	rdf:type rdfs:Class ;
	rdfs:comment "Network Intrusion Detection System. Specialised Computer objNodeect that monitors a network for malicious traffic. Defined as computer to allow access to NIDS software for consistency. Not in posession of network card to reflect assumption that it is integrated into network switch / interface. "^^xsd:string ;
	rdfs:label "Network Intrusion Detection System "^^xsd:string ;
	rdfs:subClassOf cst:Node .

cst:IdsRule 
	rdf:type rdfs:Class ;
	rdfs:comment "Intrusion Detection System Rule. A Specialised Configuration Item that is used to tune IDS'. Has properties of RuleID, Signature and Action. Currently not capable of Anomaly Detection"^^xsd:string ;
	rdfs:label "Intrusion Detection System Rule"^^xsd:string ;	
	rdfs:subClassOf cst:SoftwareConfiguration .	


#    ____    ____     ___    ____    _____   ____    _____   ___   _____   ____  
#   |  _ \  |  _ \   / _ \  |  _ \  | ____| |  _ \  |_   _| |_ _| | ____| / ___| 
#   | |_) | | |_) | | | | | | |_) | |  _|   | |_) |   | |    | |  |  _|   \___ \ 
#   |  __/  |  _ <  | |_| | |  __/  | |___  |  _ <    | |    | |  | |___   ___) |
#   |_|     |_| \_\  \___/  |_|     |_____| |_| \_\   |_|   |___| |_____| |____/ 
#                                                                                

# Properties relating to Hardware and computers

cst:hostName
	rdf:type rdf:Property ;
	rdfs:comment "Host Name of a given Computer"^^xsd:string ;
	rdfs:label "Host Name"^^xsd:string ;
	rdfs:domain cst:Computer ;
	rdfs:range xsd:string . 

cst:ipAddress
	rdf:type rdf:Property ;
	rdfs:comment "IP address of a network card"^^xsd:string ;
	rdfs:label "IP Address"^^xsd:string ;
	rdfs:domain cst:Nic ;
	rdfs:range xsd:string . 


cst:macAddress
	rdf:type rdf:Property ;
	rdfs:comment "MAC address of a network card"^^xsd:string ;
	rdfs:label "MAC Address"^^xsd:string ;
	rdfs:domain cst:Nic ;
	rdfs:range xsd:string . 


# Properties relating to networks

cst:netname
	rdf:type rdf:Property ;
	rdfs:comment "Unique name of a given network"^^xsd:string ;
	rdfs:label "Network Name"^^xsd:string ;
	rdfs:domain cst:Network ;
	rdfs:range xsd:string .

cst:routeNumber
	rdf:type rdf:Property ;
	rdfs:comment "Unique number of a route"^^xsd:string ;
	rdfs:label "Route Number"^^xsd:string ;
	rdfs:domain cst:Route ;
	rdfs:range xsd:integer .


# Properties Relating to Wireless

cst:ssid 	
	rdf:type rdf:Property ;
	rdfs:comment "Set Service Identifier. 32 Character unique identifier of Wireless Networks"^^xsd:string ;
	rdfs:label "SSID"^^xsd:string ;
	rdfs:domain cst:WirelessAccessPoint ;
	rdfs:range xsd:string .

cst:wirelessSecurityProtocolType	
	rdf:type rdf:Property ;
	rdfs:comment "Type for wireless security protocol"^^xsd:string ;
	rdfs:label "Wireless Security Protocol Type"^^xsd:string ;
	rdfs:domain cst:WirelessSecurityProtocol ;
	rdfs:range xsd:string .	

cst:wirelessSecurityProtocolStrength
	rdf:type rdf:Property ;
	rdfs:comment "Strength of the wireless security protocol"^^xsd:string ;
	rdfs:label "Wireless Security Protocol Strength"^^xsd:string ;
	rdfs:domain cst:WirelessSecurityProtocol ;
	rdfs:range xsd:string .	


# Properties relating to software and services

cst:softwareName
	rdf:type rdf:Property ;
	rdfs:comment "Name of a piece of software. Will be determined by truncating the CPE ID before the Version."^^xsd:string ;
	rdfs:label "Software Name"^^xsd:string ;
	rdfs:domain cst:Software ;
	rdfs:range xsd:string .

cst:InstalledSoftwareVersionNumber
	rdf:type rdf:Property ;
	rdfs:comment "Version number associated with a particular software version. Determined by extracting version number from CPE-ID"^^xsd:string ;
	rdfs:label "Software Version Number" ;
	rdfs:domain cst:InstalledSoftwareVersion ;
	rdfs:range xsd:string .		

cst:cpeIdentifier
	rdf:type rdf:Property ;
	rdfs:comment "Common Platform Enumeration Identifier. "^^xsd:string ;
	rdfs:label "Common Platform Enumeration Identifier" ;
	rdfs:domain cst:InstalledSoftwareVersion ;
	rdfs:range xsd:string .			

cst:servicePrivelegeLevel
	rdf:type rdf:Property ;
	rdfs:comment "Defined privilege level that the service is operating at. Define as USER, ADMINISTRATOR or SYSTEM"^^xsd:string ;
	rdfs:label "Service Privelege Level"^^xsd:string ;
	rdfs:domain cst:Service ;
	rdfs:range xsd:string .

cst:port 
	rdf:type rdf:Property ;
	rdfs:comment "Port that a remote service is running on "^^xsd:string ;
	rdfs:label "Port"^^xsd:string ;
	rdfs:domain cst:RemoteService ;
	rdfs:range xsd:int .

cst:protocol
	rdf:type rdf:Property ;
	rdfs:comment "Protocol that a remote service operates using "^^xsd:string ;
	rdfs:label "Protocol"^^xsd:string ;
	rdfs:domain cst:RemoteService ;
	rdfs:range xsd:string .	

cst:cveIdentifier
	rdf:type rdf:Property ;
	rdfs:comment "Common Vulnerability and Exposure Identifier of a vulnerability in software"^^xsd:string ;
	rdfs:label "CVE Identifier"^^xsd:string ;
	rdfs:domain cst:SoftwareVulnerability ;
	rdfs:range xsd:string .	

cst:cvssScore
	rdf:type rdf:Property ;
	rdfs:comment "The Common Vulnerability Scoring System (CVSS) score associated with a given CVE identified vulnerability. Number between 1 and 10. Measures  "^^xsd:string ;
	rdfs:label "CVSS Score"^^xsd:string ;
	rdfs:domain cst:SoftwareVulnerability ;
	rdfs:range xsd:int .	

cst:cvssExploitabilityScore
	rdf:type rdf:Property ;
	rdfs:comment "CVSS from 1 to 10 regarding the skill level required to exploit the vulnerability. 10 is most exploitable, 1 is least."^^xsd:string ;
	rdfs:label "CVSS Exploitability Score"^^xsd:string ;
	rdfs:domain cst:SoftwareVulnerability ;
	rdfs:range xsd:int ;
	rdfs:subPropertyOf cst:cvssScore .

cst:cweIdentifier
	rdf:type rdf:Property ;
	rdfs:comment "The Common Weakness Enumeration (CWE) score associated with a given CVE identified vulnerability. Categorises Vulnerabilities into logical Groupings."^^xsd:string ;
	rdfs:label "CWE Score"^^xsd:string ;
	rdfs:domain cst:SoftwareWeakness ;
	rdfs:range xsd:int .	


# The Following Properties relate to Domains and Users

cst:domainName
	rdf:type rdf:Property ;
	rdfs:comment "Unique name of a domain"^^xsd:string ;
	rdfs:label "Domain Name"^^xsd:string ;
	rdfs:domain cst:Domain ;
	rdfs:range xsd:string .

cst:userID
	rdf:type rdf:Property ;
	rdfs:comment "Unique Identifier of a User"^^xsd:string ;
	rdfs:label "User ID"^^xsd:string ;
	rdfs:domain cst:User ;
	rdfs:domain xsd:string .

cst:username
	rdf:type rdf:Property ;
	rdfs:comment "Name of account"^^xsd:string ;
	rdfs:label "Username"^^xsd:string ;
	rdfs:domain cst:User ;
	rdfs:range xsd:string .

cst:password 
	rdf:type rdf:Property ;
	rdfs:comment "Password of user. Required for Authentication"^^xsd:string ;
	rdfs:label "Password"^^xsd:string ;
	rdfs:domain cst:User ;
	rdfs:range xsd:string .

cst:userPrivilegeLevel
	rdf:type rdfs:Property ;
	rdfs:comment "user's privilege level. Must be either USER or ADMINISTRATOR"^^xsd:string ;
	rdfs:label "User Privilege Level"^^xsd:string ;
	rdfs:domain cst:User ;
	rdfs:range xsd:string .

# The Following Properties relate to Disks Data and Encryption

cst:diskSize
	rdf:type rdf:Property ;
	rdfs:comment "Size of Disk (I.e. Data Capacity)"^^xsd:string ;
	rdfs:label "Disk Size"^^xsd:string ;
	rdfs:domain cst:Disk ;
	rdfs:range xsd:int .

cst:volumeName 
	rdf:type rdfs:Property ;
	rdfs:comment "Name associated with a disk"^^xsd:string ;
	rdfs:label "Volume Name"^^xsd:string ;
	rdfs:domain cst:Disk ;
	rdfs:range xsd:string .

cst:enryptionAlgorithim
	rdf:type rdf:Property ;
	rdfs:comment "The Algorithim used to encrypt a disk"^^xsd:string ;
	rdfs:label "Encryption Algorithim"^^xsd:string ;
	rdfs:domain cst:Encryption ;
	rdfs:range xsd:string .

cst:encryptionKeyLength
	rdf:type rdf:Property ;
	rdfs:comment "The Keylength of the Encryption algorithim - relates to strength of encryption algorithim "^^xsd:string ;
	rdfs:label "Encryption Key Length"^^xsd:string ;
	rdfs:domain cst:Encryption ;
	rdfs:range xsd:int .

cst:dataSize 
	rdf:type rdf:Property ;
	rdfs:comment "Size of a given piece of data"^^xsd:string ;
	rdfs:label "Size of Data Item"^^xsd:string ;
	rdfs:domain cst:Data ;
	rdfs:range xsd:int .

cst:dataType 
	rdf:type rdf:Property ;
	rdfs:comment "the Type, or nature of the data"^^xsd:string ;
	rdfs:label "Type of Data"^^xsd:string ;
	rdfs:domain cst:Data ;
	rdfs:range xsd:string .				


# Properties Relating to IDS

cst:ruleNumber 
	rdf:type rdf:Property ;
	rdfs:comment "The unique identifier of the IDS rule"^^xsd:string ;
	rdfs:label "Intrusion Detection System Rule Number"^^xsd:string ;
	rdfs:domain cst:IdsRule ;
	rdfs:range xsd:string .

cst:idsSignature
	rdf:type rdf:Property ;
	rdfs:comment "A Signature that will be used to trigger an IDS. Will be associated with the Exploit ID or CVE etc of a malicious activity. Allows the instantiator to define their 'database of known attacks' and simulate 0-days"^^xsd:string ;
	rdfs:label "IDS Signature"^^xsd:string ;
	rdfs:domain cst:IdsRule ;
	rdfs:range xsd:string .
	# Mapping of Vulns to Exploits https://cve.mitre.org/data/refs/refmap/source-EXPLOIT-DB.html

cst:idsAction 
	rdf:type rdf:Property ;
	rdfs:comment "The Action to be taken by the IDS. Could be 'alert' 'ignore' 'activate MTNDM' etc. Enalbes the instantiator to replicate poorly designed or tuned IDS"^^xsd:string ;
	rdfs:label "IDS Action"^^xsd:string ;
	rdfs:domain cst:IdsRule ; 
	rdfs:range xsd:string .		


#    ____    _____   _          _      _____   ___    ___    _   _   ____    _   _   ___   ____    ____  
#   |  _ \  | ____| | |        / \    |_   _| |_ _|  / _ \  | \ | | / ___|  | | | | |_ _| |  _ \  / ___| 
#   | |_) | |  _|   | |       / _ \     | |    | |  | | | | |  \| | \___ \  | |_| |  | |  | |_) | \___ \ 
#   |  _ <  | |___  | |___   / ___ \    | |    | |  | |_| | | |\  |  ___) | |  _  |  | |  |  __/   ___) |
#   |_| \_\ |_____| |_____| /_/   \_\   |_|   |___|  \___/  |_| \_| |____/  |_| |_| |___| |_|     |____/ 
#                                                                                                        

# Regarding Core Computer and Network Functionality

cst:hasNic
	rdf:type rdf:Property ;
	rdfs:comment "Link between computer and network card"^^xsd:string ;
	rdfs:label "Has Network Card"^^xsd:string ;
	rdfs:domain cst:Computer ;
	rdfs:range cst:Nic .

cst:isConnectedTo
	rdf:type rdf:Property ;
	rdf:type owl:TransitiveProperty ;
	owl:disjointUnionOf (cst:Nic cst:WirelessAccessPoint) ;
	rdfs:comment "Link between NIC and WAP and Network"^^xsd:string ;
	rdfs:label "Is Connected To"^^xsd:string ;
	rdfs:domain cst:Nic ;
	rdfs:range cst:WirelessAccessPoint ;
	rdfs:domain cst:WirelessAccessPoint ;
	rdfs:range cst:Network .	

cst:hasEdgeNic
	rdf:type rdf:Property ;
	rdfs:comment "Link to network interface on router"^^xsd:string ;
	rdfs:label "Edge Network Interface"^^xsd:string ;
	rdfs:domain cst:Network ;
	rdfs:range cst:Nic .

cst:hasRoute
	rdf:type rdf:Property ;
	rdfs:comment "A route between networks posessed by a router"^^xsd:string ;
	rdfs:label "Has Route"^^xsd:string ;
	rdfs:domain cst:Router ;
	rdfs:range cst:Route .	

cst:routeOrigin
	rdf:type rdf:Property ;
	rdfs:comment "Start point of a route"^^xsd:string ;
	rdfs:label "Route Origin"^^xsd:string ;
	rdfs:domain cst:Route ;
	rdfs:range cst:Nic .

cst:routeDestination
	rdf:type rdf:Property ;
	rdfs:comment "End point of a route"^^xsd:string ;
	rdfs:label "Route Destination"^^xsd:string ;
	rdfs:domain cst:Route ;
	rdfs:range cst:Nic .


# The Following Relationships regard Wireless

cst:hasWirelessSecurityProtocol
	rdf:type rdf:Property ;
	rdfs:comment "Links to the wireless security protocol running on a given wireless access point"^^xsd:string ;
	rdfs:label "Has Wireless Security Protocol"^^xsd:string ;
	rdfs:domain cst:WirelessAccessPoint ;
	rdfs:range cst:WirelessSecurityProtocol .


# Regarding Virtualisation 

cst:hasVirtualNIC
	rdf:type rdf:Property ;
	rdfs:comment "Denotes conenction to a VNIC. Facilitates the differentiation of physical and virtual machines when querying the network. "^^xsd:string ;
	rdfs:label "Has Virtual NIC"^^xsd:string ;
	rdfs:domain cst:VirtualMachine ;
	rdfs:range cst:VirtualNic .		
	#This propery exists in order to facilitate the differentiation of VM to VNIC and Physical computer to VNIC connections in querying. 

cst:hasVirtualPrivateNetworkConnection
	rdf:type rdf:Property ;
	rdfs:comment "Denotes a VPN connection to a subnet"^^xsd:string ;
	rdfs:label "Has Virtual Private Network Connection"^^xsd:string ;
	rdfs:domain cst:VirtualNic ;
	rdfs:range cst:SubNetwork .		

cst:isVirtuallyConnectedTo
	rdf:type rdf:Property ;
	rdfs:comment "Link between NIC and Network"^^xsd:string ;
	rdfs:label "Is Virtually Connected To"^^xsd:string ;
	rdfs:domain cst:VirtualNic ;
	rdfs:range cst:VirtualNetwork .	


# Following relationships are to do with software, services and vulnerabilities. 

cst:isSoftwareType 
	rdf:type rdf:Property ;
	rdfs:comment "A node can run zero to many pieces of software"^^xsd:string ;
	rdfs:label "Has Software Type."^^xsd:string ;
	rdfs:domain cst:InstalledSoftwareVersion ;
	rdfs:range cst:SoftwareType .

cst:hasInstalledSoftwareVersion
	rdf:type rdf:Property ;
	rdfs:comment "A node can run zero to many of installed software versions"^^xsd:string ;
	rdfs:label "Has Installed Software."^^xsd:string ;
	rdfs:domain cst:Node ;
	rdfs:range cst:InstalledSoftwareVersion .	

cst:projectsService 
	rdf:type rdf:Property ;
	rdfs:comment "Software will project a service onto the computer either locally or remotely."^^xsd:string ;
	rdfs:label "Projects Service "^^xsd:string ;
	rdfs:domain cst:InstalledSoftwareVersion ;
	rdfs:range cst:Service .

cst:hasVisibleService
	rdf:type rdf:Property ;
	rdfs:comment "A remote service is visible on a computers network card (IOT facilitate port scanning and attack vectors"^^xsd:string ;
	rdfs:label "Is Visible On"^^xsd:string ;
	rdfs:domain cst:Nic ;
	rdfs:range cst:RemoteService .	

cst:hasSoftwareVulnerability
	rdf:type rdf:Property ;
	rdfs:comment "A Software Version will be associated with between zero and many vulnerabilities"^^xsd:string ;
	rdfs:label "Has Vulnerability"^^xsd:string ;
	rdfs:domain cst:InstalledSoftwareVersion ;
	rdfs:range cst:SoftwareVulnerability .

cst:includesVulnerability 
	rdf:type rdf:Property ;
	rdfs:comment "The Vulnerabilites included in a weakness"^^xsd:string ;
	rdfs:label "Includes Vulnerability"^^xsd:string ;
	rdfs:domain cst:SoftwareWeakness ;
	rdfs:range cst:SoftwareVulnerability .

cst:hasSoftwareConfiguration 
	rdf:type rdf:Property ;
	rdfs:comment "The Association between a software configuration and it's version"^^xsd:string ;
	rdfs:label "Has Software Configuration"^^xsd:string ;
	rdfs:domain cst:InstalledSoftwareVersion ;
	rdfs:range cst:SoftwareConfiguration .	


# The Following relationships are regarding Domains and Users

cst:controlsDomain
	rdf:type rdf:Property ;
	rdfs:comment "Link between the domain controller and the domain "^^xsd:string ;
	rdfs:label "Controls Domain "^^xsd:string ;
	rdfs:domain cst:DomainController ;
	rdfs:range cst:Domain .

cst:hasAccessTo 
	rdf:type rdf:property ;
	rdf:type owl:TransitiveProperty ;
	owl:disjointUnionOf (cst:LocalUser cst:DomainUser cst:Domain) ;
	rdfs:comment "Transitive Property to determine the users assocaited with a computer"^^xsd:string ;
	rdfs:label "Has Access To"^^xsd:string ;
	rdfs:domain cst:LocalUser ;
	rdfs:range cst:Computer ;
	rdfs:domain cst:DomainUser ;
	rdfs:range cst:Domain ;
	rdfs:domain cst:Domain .
	#Disjoint union adresses the multiple domains in this relationship


# The following relationships are to do with Disks, Data and Encryption

cst:hasDisk
	rdf:type rdf:Property ;
	rdfs:comment "Relationship between disk and a computer. A computer can have multiple disks "^^xsd:string ;
	rdfs:label "Has Disk"^^xsd:string ;
	rdfs:domain cst:Computer ;
	rdfs:range cst:Disk .

cst:isEncryptedWith
	rdf:type rdf:Property ;
	rdfs:comment "Link between a disk and its encryption. If no encryption the relationship won't be made"^^xsd:string ;
	rdfs:label "Is Encrypted With"^^xsd:string ;
	rdfs:domain cst:Disk ;
	rdfs:range cst:Encryption .

cst:containsData 
	rdf:type rdf:Property ;
	rdfs:comment "Relationship between disk and data. Can have multiple pieces of data on a disk. Data size should not exceed disk size"^^xsd:string ;
	rdfs:label "Contains Data"^^xsd:string ;	
	rdfs:domain cst:Disk ;
	rdfs:range cst:Data .

cst:hasOwner
	rdf:type rdf:Property ;
	rdfs:comment "Data is owned by someone. If the person trying to access the data is not the owner then they should be denied access alt: encryption should be activated "^^xsd:string ;
	rdfs:label "Has Owner"^^xsd:string ;
	rdfs:domain cst:Data ;
	rdfs:range cst:User .


#The Following Relationships are related to the implementation of IDS 

cst:monitorsSubnet 
	rdf:type rdf:Property ;
	rdfs:comment "The NIDS will monitor a subnet."^^xsd:string ;
	rdfs:label "monitors Subnet"^^xsd:string ;
	rdfs:domain cst:NetworkIDS ;
	rdfs:range cst:SubNetwork .

	



